行政機関や人材プールを表現するsubStateを実装

GSM.v
@@ -3,13 +3,12 @@ Export RecordSetNotations.
 From mathcomp Require Export all_ssreflect.
 Require Export Nat.
 
-
 Set Implicit Arguments.
 Unset Strict Implicit.
 
-(***************)
-(* パラメータなど *)    
-(***************)
+(********************)
+(* メタ・アサンプション *)
+(********************)
 
 Parameter citizen : finType.
 Definition currency := nat.
@@ -22,99 +21,158 @@ Definition randomC := random_choice citizen.
 Definition randomSetC := random_choice {set citizen}.
 
 
-(*******)
-(* 役職 *)    
-(*******)
 
-Variant role :=
-    | Professional
-    | Facilitator.
+Variant admin :=
+    | global    
+    | police
+    | judiciary
+    | military 
+    | media
+    | education
+    | registration
+    | professional
+    | facilitator.
 
-Lemma eq_role_dec (s t : role) : { s = t} + { s <> t}.
-Proof. decide equality; apply eq_comparable. Qed.
-Definition role_eqMixin := EqMixin (compareP eq_role_dec).
-Canonical Structure role_eqType := Eval hnf in @EqType role role_eqMixin.
 
 (************)
 (* アクション *)
 (************)
 
 Inductive proposal  :=
-    | Passign : role -> citizen -> proposal
-    | Pdismissal : role -> citizen -> proposal
-    | Padd_mem :citizen -> proposal
-    | Pdel_mem :citizen -> proposal 
+    | Passign : admin -> citizen -> proposal
+    | Pdismissal : admin -> citizen -> proposal
     | Pwithdraw : currency -> proposal 
     | Pdeposit : currency -> proposal 
-    | Pallocate : currency -> role -> proposal
-    | Pset_expiration : role -> timestamp -> proposal.
+    | Pallocate : admin -> currency ->  proposal
+    | Pset_tenure : admin -> citizen -> proposal
+    | Pset_expiration : admin -> timestamp -> proposal.    
 
-Lemma eq_proposal_dec (s t : proposal) : { s = t} + { s <> t}.
-Proof. decide equality; apply eq_comparable. Qed.
-Definition proposal_eqMixin := EqMixin (compareP eq_proposal_dec).
-Canonical Structure proposal_eqType := Eval hnf in @EqType proposal proposal_eqMixin.
 
 Inductive act :=
-    | Apropose : proposal -> random -> random -> random -> act
-    | Adeliberate.
+    | Apropose : admin -> proposal -> random -> random -> random -> act
+    | Adeliberate : admin -> act.
 
 
 (************)    
 (* 状態と熟議 *)
 (************)
 
+
+
 Record deliberation := mkDlb{
     Dproposal : proposal;
     Dprofessional : citizen;
     Dfacilitator : citizen;
-    Ddeliberator : {set citizen};
+    Ddeliberator : {set citizen};    
 }.
+
+
+
+Record subState := mkSubState{
+    SSbudget : currency;
+    SStenure : option citizen;
+    SSterm : timestamp;
+    SSmember : {set citizen};
+    SSdeliberation : option deliberation
+}.
+
 
 Record state := mkState{
     Streasury : currency;    
-    Smember : {set citizen};
-    Sassignment : role -> {set citizen};
-    Sbudget : role -> currency;
-    Sexpiration : role -> timestamp;
-    Sdeliberation : deliberation
+    Sadmin : admin -> subState;    
 }.
+
+(*********************)
+(* updatable recortd *)
+(*********************)
+
+
+Instance etaSubState : Settable subState := 
+    settable! mkSubState 
+        < SSbudget; SStenure; SSterm; SSmember; SSdeliberation>.
 
 Instance etaState : Settable state := 
     settable! mkState 
-        < Streasury; Smember; Sassignment; Sbudget; Sexpiration; Sdeliberation >.
+        < Streasury; Sadmin >.
+
+
+
+
+(**************************)
+(* eqType's instantiation *)
+(**************************)
+
+Tactic Notation "mkCompEq"  :=
+    refine (EqMixin (compareP _)) => x y;
+    unfold decidable; decide equality; apply eq_comparable.
+
+Definition eqMixin := Equality.mixin_of.
+
+Definition admin_eqMixin : eqMixin admin. Proof. mkCompEq. Qed.
+Canonical Structure admin_eqType := Eval hnf in @EqType admin admin_eqMixin.
+
+Definition proposal_eqMixin : eqMixin proposal. Proof. mkCompEq. Qed.
+Canonical Structure proposal_eqType := Eval hnf in @EqType proposal proposal_eqMixin.
+
+
+Definition deliberation_eqMixin  : eqMixin deliberation. Proof. mkCompEq. Qed.
+Canonical Structure deliberation_eqType := Eval hnf in @EqType deliberation deliberation_eqMixin.        
+
+Definition subState_eqMixin : eqMixin subState. Proof. mkCompEq. Qed.
+Canonical Structure subState_eqType := Eval hnf in @EqType subState subState_eqMixin.
 
 
 (**********)
 (* 状態遷移 *)
 (**********)
 
+Definition subst {dom : eqType} {ran} (d : dom) (r : ran) := 
+    fun f => fun d' =>  if d == d' then r else f d'.
+Notation "a ↦ b" := (subst a b)(at level 10).
+
 Parameter evalD : deliberation -> bool.  
 
 Definition transv_  (a : proposal) (x : state)  :=
-    match a with 
-    | Passign r m => 
-        x <| Sassignment ::= fun f => fun r' => if r == r' then m |: f r' else f r' |>
-    | Pdismissal r m => 
-        x <| Sassignment ::= fun f => fun r' => if r == r' then f r' :\ m else f r' |> 
-
-    | Padd_mem m => x <| Smember ::= fun X => m |: X|>
-    | Pdel_mem m => x <| Smember ::= fun X => X :\ m|>
-
+    match a with     
     | Pwithdraw n => x <|Streasury ::= plus n|>    
     | Pdeposit n => x <|Streasury ::= minus n|>
-    | Pallocate n r => x <|Streasury ::= minus n|> 
-                        <|Sbudget ::= fun f => fun r' => if r == r' then f r + n else f r'|>
-
-    | Pset_expiration r n => 
-        x  <|Sbudget ::= fun f => fun r' => if r == r' then n else f r'|>                   
+    | Passign a m => 
+        let ss := Sadmin x a in 
+        let ss' := ss <| SSmember ::= fun mem => m |: mem |> in
+        x <| Sadmin ::= a ↦ ss'|>
+    | Pdismissal a m => 
+        let ss := Sadmin x a in 
+        let ss' := ss <| SSmember ::= fun mem => mem :\ m |> in
+        x <| Sadmin ::= a ↦ ss'|>
+    | Pallocate a n => 
+        let ss := Sadmin x a in 
+        let ss' := ss <| SSbudget ::= fun n' => n + n' |> in
+        x <| Sadmin ::= a ↦ ss'|>
+    | Pset_tenure a m => 
+        let ss := Sadmin x a in 
+        let ss' := ss <| SStenure := Some m |> in
+        x <| Sadmin ::= a ↦ ss'|>
+    | Pset_expiration a n =>
+        let ss := Sadmin x a in 
+        let ss' := ss <| SSterm := n |> in
+        x <| Sadmin ::= a ↦ ss'|>
     end.
+
 
 Definition trans_ (a : act) (x : state) :=
     match a with 
-    | Apropose a' p_ f_ d_ => 
-        x <| Sdeliberation := mkDlb a' (randomC p_) (randomC f_ ) (randomSetC d_) |>
-    | Adeliberate => 
-        if evalD (Sdeliberation x) then transv_ (Dproposal (Sdeliberation x)) x else x
+    | Apropose adm a' p_ f_ d_ => 
+        let ss := Sadmin x adm in         
+        let ss' := ss <|SSdeliberation := Some (mkDlb a' (randomC p_) (randomC f_ ) (randomSetC d_))|> in 
+        x <| Sadmin ::= adm ↦ ss'|>
+    | Adeliberate adm => 
+        let ss := Sadmin x adm in
+        let dlb_ := SSdeliberation ss in
+        match dlb_ with 
+        | Some  dlb =>  
+            if evalD dlb then transv_ (Dproposal dlb) x else x
+        | None => x
+        end
     end.
 
 
@@ -125,22 +183,60 @@ Definition trans a x y := y = trans_ a x.
 (***********)
 
 Inductive var :=
-    | isAssigned : role -> citizen -> var
-    | isMember : citizen -> var
-    | withinTerm : role -> var
-    | isProposed : proposal -> var
-    | isValidDeliberation.
+    | isAssigned : admin -> citizen -> var
+    | withinTerm : admin -> var
+    | isProposed : admin -> proposal -> var
+    | hasTenuren : admin -> var
+    | isTenuren : admin -> citizen -> var
+    | isValidDeliberation : admin -> var.
+
+
+
 
 Definition valuation (x : var) (s : state) : bool :=
-    match x with 
-    | isAssigned r m => m \in Sassignment s r
-    | isMember m => m \in Smember s
-    | withinTerm r => now <? Sexpiration s r 
-    | isProposed a => a == Dproposal (Sdeliberation s)
-    | isValidDeliberation => 
-        (Dprofessional (Sdeliberation s) \in Sassignment s Professional) && 
-        (Dfacilitator (Sdeliberation s) \in Sassignment s Facilitator) &&
-        (Ddeliberator (Sdeliberation s) != set0)
+    match x with     
+    | isAssigned a m => 
+        let ss := Sadmin s a in 
+        let mem := SSmember ss in         
+        m \in mem
+    | withinTerm a => 
+        let ss := Sadmin s a in 
+        let n := SSterm ss in
+        now <? n
+    | isProposed adm a => 
+        let ss := Sadmin s adm in 
+        let dlb_ := SSdeliberation ss in
+        match dlb_ with 
+        | Some  dlb =>  
+            a == Dproposal dlb
+        | None => false
+        end
+    | isValidDeliberation a => 
+        let ss := Sadmin s a in 
+        let ps := SSmember (Sadmin s professional) in 
+        let fs := SSmember (Sadmin s facilitator) in 
+        let dlb_ := SSdeliberation ss in
+        match dlb_ with 
+        | Some  dlb =>  
+            (Dprofessional dlb \in ps) && 
+            (Dfacilitator dlb \in fs) &&
+            (Ddeliberator dlb != set0)
+        | None => false
+        end        
+    | hasTenuren a => 
+        let ss := Sadmin s a in 
+        let m := SStenure ss in 
+        match m with 
+        | Some _ => true 
+        | _ => false 
+        end
+    | isTenuren a m  =>
+        let ss := Sadmin s a in 
+        let m' := SStenure ss in 
+        match m' with 
+        | Some m'' => m'' == m 
+        | _ => false
+        end
     end.
 
 
